src/compiler/meta/OCL_compiler_meta_Isabelle.thy
@@ -58,27 +58,19 @@ datatype hol_dataty = Datatype string (* name *)
 
 datatype hol_raw_ty =
    Ty_apply hol_raw_ty "hol_raw_ty list"
+ | Ty_apply_bin string (* binop *) hol_raw_ty hol_raw_ty
  | Ty_base string
- | Ty_arrow hol_raw_ty hol_raw_ty
- | Ty_times hol_raw_ty hol_raw_ty
 
 datatype hol_ty_synonym = Type_synonym string (* name *)
                                        hol_raw_ty (* content *)
 
-datatype hol_expr = Expr_case hol_expr (* value *)
-                              "(hol_expr (* pattern *) \<times> hol_expr (* to return *)) list"
-                  | Expr_rewrite hol_expr (* left *) string (* symb rewriting *) hol_expr (* right *)
+datatype hol_expr = Expr_rewrite hol_expr (* left *) string (* symb rewriting *) hol_expr (* right *)
                   | Expr_basic "string list"
                   | Expr_oid string (* prefix *) internal_oid
-                  | Expr_binop hol_expr string hol_expr
                   | Expr_annot0 hol_expr hol_raw_ty
-                  | Expr_bind string (* symbol *) "string list" (* arg *) hol_expr
                   | Expr_bind0 string (* symbol *) hol_expr (* arg *) hol_expr
-                  | Expr_function "(hol_expr (* pattern *) \<times> hol_expr (* to return *)) list"
-                  | Expr_apply string "hol_expr list"
-                  | Expr_applys hol_expr "hol_expr list"
-                  | Expr_preunary hol_expr hol_expr (* no parenthesis and separated with one space *)
-                  | Expr_postunary hol_expr hol_expr (* no parenthesis and separated with one space *)
+                  | Expr_function0 "hol_expr (* value *) option" (* none: function *) "(hol_expr (* pattern *) \<times> hol_expr (* to return *)) list"
+                  | Expr_applys00 hol_expr "hol_expr list"
                   | Expr_paren string (* left *) string (* right *) hol_expr
                   | Expr_if_then_else hol_expr hol_expr hol_expr
                   | Expr_inner pure_term (* inner syntax term *)
@@ -105,38 +97,43 @@ datatype hol_ntheorem = Thm_str string
                       | Thm_of hol_ntheorem "hol_expr list"
                       | Thm_OF hol_ntheorem hol_ntheorem
 
-datatype hol_lemmas_simp = Lemmas_simp string (* name *)
-                                       "hol_ntheorem list"
-                         | Lemmas_nosimp string (* name *)
+datatype hol_ntheorems = Thms_single hol_ntheorem
+                       | Thms_mult string
+
+type_synonym hol_ntheorems_l = "hol_ntheorems list"
+
+datatype hol_lemmas_simp = Lemmas_simp_opt
+                                       bool (* True : simp *)
+                                       string (* name *)
                                        "hol_ntheorem list"
                          | Lemmas_simps string (* name *)
                                         "string (* thms *) list"
 
-datatype hol_tactic = Tac_rule hol_ntheorem
-                    | Tac_drule hol_ntheorem
-                    | Tac_erule hol_ntheorem
-                    | Tac_intro "hol_ntheorem list"
-                    | Tac_elim hol_ntheorem
-                    | Tac_subst_l "string (* nat *) list" (* pos *) hol_ntheorem
-                    | Tac_insert "hol_ntheorem list"
-                    | Tac_plus "hol_tactic list"
-                    | Tac_option "hol_tactic list"
-                    | Tac_simp | Tac_simp_add2 "string list" (* thms *) "string list" (* thm *) | Tac_simp_add_del "string list" "string list" | Tac_simp_only "hol_ntheorem list" | Tac_simp_add0 "hol_ntheorem list"
-                    | Tac_simp_all | Tac_simp_all_add string
-                    | Tac_auto_simp_add2 "string list" (* thms *)
-                                         "string list" (* thm *)
-                    | Tac_auto_simp_add_split "hol_ntheorem list" "string list"
-                    | Tac_rename_tac "string list"
-                    | Tac_case_tac hol_expr
-                    | Tac_blast "nat option"
+datatype hol_tactic_simp = Simp_only hol_ntheorems_l
+                         | Simp_add_del hol_ntheorems_l (* add *) hol_ntheorems_l (* del *)
+
+datatype hol_tactic = Tact_rule hol_ntheorem
+                    | Tact_drule hol_ntheorem
+                    | Tact_erule hol_ntheorem
+                    | Tact_intro "hol_ntheorem list"
+                    | Tact_elim hol_ntheorem
+                    | Tact_subst_l "string (* nat *) list" (* pos *) hol_ntheorem
+                    | Tact_insert hol_ntheorems_l
+                    | Tact_plus "hol_tactic list"
+                    | Tact_option "hol_tactic list"
+                    | Tact_one hol_tactic_simp
+                    | Tact_auto_simp_add_split hol_ntheorems_l "string list"
+                    | Tact_rename_tac "string list"
+                    | Tact_case_tac hol_expr
+                    | Tact_blast "nat option"
 
 datatype hol_tactic_last = Tacl_done
                          | Tacl_by "hol_tactic list"
                          | Tacl_sorry
 
 datatype hol_tac_apply = App "hol_tactic list" (* apply (... ',' ...) *)
-                       | App_using "hol_ntheorem list" (* using ... *)
-                       | App_unfolding "hol_ntheorem list" (* unfolding ... *)
+                       | App_using0 hol_ntheorems_l (* using ... *)
+                       | App_unfolding0 hol_ntheorems_l (* unfolding ... *)
                        | App_let hol_expr (* name *) hol_expr
                        | App_have string (* name *) hol_expr hol_tactic_last
                        | App_fix "string list"
@@ -181,6 +178,7 @@ section{* ... *}
 definition "thm_OF s l = List.fold (\<lambda>x acc. Thm_OF acc x) l s"
 definition "thm_simplified s l = List.fold (\<lambda>x acc. Thm_simplified acc x) l s"
 definition "Expr_annot e s = Expr_annot0 e (Ty_base s)"
+definition "Expr_bind symb s e = Expr_bind0 symb (Expr_basic s) e"
 definition "Expr_lambdas = Expr_bind unicode_lambda"
 definition "Expr_lambda x = Expr_lambdas [x]"
 definition "Expr_lambdas0 = Expr_bind0 unicode_lambda"
@@ -191,6 +189,7 @@ definition "Expr_warning_parenthesis (* optional parenthesis that can be removed
 definition "Expr_pat b = Expr_basic [Char Nibble3 NibbleF # b]"
 definition "Expr_And x f = Expr_bind0 unicode_And (Expr_basic [x]) (f x)"
 definition "Expr_exists x f = Expr_bind0 unicode_exists (Expr_basic [x]) (f x)"
+definition "Expr_binop = Expr_rewrite"
 definition "expr_binop s l = (case rev l of x # xs \<Rightarrow> List.fold (\<lambda>x. Expr_binop x s) xs x)"
 definition "expr_binop' s l = (case rev l of x # xs \<Rightarrow> List.fold (\<lambda>x. Expr_parenthesis o Expr_binop x s) xs x)"
 definition "Expr_set l = (case l of [] \<Rightarrow> Expr_basic [''{}''] | _ \<Rightarrow> Expr_paren ''{'' ''}'' (expr_binop '','' l))"
@@ -199,6 +198,15 @@ definition "Expr_list l = (case l of [] \<Rightarrow> Expr_basic [''[]''] | _ \<
 definition "Expr_list' f l = Expr_list (List_map f l)"
 definition "Expr_pair e1 e2 = Expr_parenthesis (Expr_binop e1 '','' e2)"
 definition "Expr_string s = Expr_basic [flatten [[Char Nibble2 Nibble2], s, [Char Nibble2 Nibble2]]]"
+definition "Expr_applys0 e l = Expr_parenthesis (Expr_applys00 e (List_map Expr_parenthesis l))"
+definition "Expr_applys e l = Expr_applys0 (Expr_parenthesis e) l"
+definition "Expr_apply e = Expr_applys0 (Expr_basic [e])"
+definition "Expr_preunary e1 e2 = Expr_applys00 e1 [e2]" (* no parenthesis and separated with one space *)
+definition "Expr_postunary e1 e2 = Expr_applys00 e1 [e2]" (* no parenthesis and separated with one space *)
+definition "Expr_case = Expr_function0 o Some"
+definition "Expr_function = Expr_function0 None"
+definition "Lemmas_simp = Lemmas_simp_opt True"
+definition "Lemmas_nosimp = Lemmas_simp_opt False"
 definition "Consts_value = ''(_)''"
 definition "Consts_raw0 s l e o_arg = Consts_raw s l (e @@ (case o_arg of
          None \<Rightarrow> ''''
@@ -208,11 +216,42 @@ definition "Consts_raw0 s l e o_arg = Consts_raw s l (e @@ (case o_arg of
                 ''''
               else
                 Consts_value @@ (flatten (List_map (\<lambda>_. '','' @@ Consts_value) (List_upto 2 arg))))))"
+definition "Ty_arrow = Ty_apply_bin unicode_Rightarrow"
+definition "Ty_times = Ty_apply_bin unicode_times"
 definition "Consts s l e = Consts_raw0 s (Ty_arrow (Ty_base (Char Nibble2 Nibble7 # unicode_alpha)) l) e None"
-definition "Tac_subst = Tac_subst_l [''0'']"
+definition "Tac_rule = Tact_rule"
+definition "Tac_drule = Tact_drule"
+definition "Tac_erule = Tact_erule"
+definition "Tac_intro = Tact_intro"
+definition "Tac_elim = Tact_elim"
+definition "Tac_subst_l = Tact_subst_l"
+definition "Tac_insert = Tact_insert o List_map Thms_single"
+definition "Tac_plus = Tact_plus"
+definition "Tac_option = Tact_option"
+definition "Tac_simp = Tact_one (Simp_add_del [] [])"
+definition "Tac_simp_add2 l1 l2 = Tact_one (Simp_add_del (flatten [ List_map Thms_mult l1
+                                                                  , List_map (Thms_single o Thm_str) l2])
+                                                         [])"
+definition "Tac_simp_add_del l1 l2 = Tact_one (Simp_add_del (List_map (Thms_single o Thm_str) l1)
+                                                            (List_map (Thms_single o Thm_str) l2))"
+definition "Tac_simp_only l = Tact_one (Simp_only (List_map Thms_single l))"
+definition "Tac_simp_add0 l = Tact_one (Simp_add_del (List_map Thms_single l) [])"
 definition "Tac_simp_add = Tac_simp_add2 []"
+definition "Tac_simp_all = Tac_plus [Tac_simp]"
+definition "Tac_simp_all_add s = Tac_plus [Tac_simp_add [s]]"
+definition "Tac_auto_simp_add2 l1 l2 = Tact_auto_simp_add_split (flatten [ List_map Thms_mult l1
+                                                                , List_map (Thms_single o Thm_str) l2]) []"
+definition "Tac_auto_simp_add_split l = Tact_auto_simp_add_split (List_map Thms_single l)"
+definition "Tac_rename_tac = Tact_rename_tac"
+definition "Tac_case_tac = Tact_case_tac"
+definition "Tac_blast = Tact_blast"
+
+definition "Tac_subst = Tac_subst_l [''0'']"
 definition "Tac_auto_simp_add = Tac_auto_simp_add2 []"
 definition "Tac_auto = Tac_auto_simp_add []"
 definition "ty_arrow l = (case rev l of x # xs \<Rightarrow> List.fold Ty_arrow xs x)"
+
+definition "App_using = App_using0 o List_map Thms_single"
+definition "App_unfolding = App_unfolding0 o List_map Thms_single"
 
 end
